erasure/theories/Erasure.v
@@ -1,25 +1,17 @@
 (* Distributed under the terms of the MIT license. *)
 From Coq Require Import Program ssreflect ssrbool.
-From Equations Require Import Equations.
-From MetaCoq.Template Require Import Transform bytestring config utils BasicAst uGraph.
-From MetaCoq.Template Require Pretty Environment Typing WcbvEval EtaExpand.
-Set Warnings "-notation-overridden".
-From MetaCoq.PCUIC Require PCUICAst PCUICAstUtils PCUICTyping
-     TemplateToPCUIC TemplateToPCUICCorrectness TemplateToPCUICWcbvEval TemplateToPCUICExpanded.
-From MetaCoq.PCUIC Require PCUICExpandLets PCUICExpandLetsCorrectness.
-Set Warnings "+notation-overridden".
-From MetaCoq.SafeChecker Require Import PCUICErrors PCUICWfEnvImpl.
+From MetaCoq.Template Require Import Transform bytestring config utils.
+From MetaCoq.PCUIC Require PCUICAst PCUICAstUtils PCUICProgram.
 From MetaCoq.Erasure Require EAstUtils ErasureFunction ErasureCorrectness EPretty Extract.
-From MetaCoq.Erasure Require ErasureFunction EOptimizePropDiscr ERemoveParams EWcbvEval EDeps.
+From MetaCoq.Erasure Require Import ETransform.
+
+Import PCUICProgram.
+Import TemplateProgram (template_eta_expand).
+Import PCUICTransform (template_to_pcuic_transform, pcuic_expand_lets_transform).
+
 Import bytestring.
 Local Open Scope bs.
 Local Open Scope string_scope2.
-
-#[local] Instance extraction_checker_flags : checker_flags := 
-  {| check_univs := true;
-     prop_sub_type := false;
-     indices_matter := false;
-     lets_in_constructor_types := true |}.
 
 (* This is the total erasure function +
   let-expansion of constructor arguments and case branches +
@@ -27,558 +19,54 @@ Local Open Scope string_scope2.
   the optimization that removes all pattern-matches on propositions. *)
 
 Import Transform.
-Obligation Tactic := idtac.
 
 Obligation Tactic := program_simpl.
 
-Definition build_wf_env_from_env {cf : checker_flags} (Σ : global_env_map) (wfΣ : ∥ wf Σ ∥) : wf_env := 
-  {| wf_env_referenced := {| referenced_impl_env := Σ.(trans_env_env); referenced_impl_wf := wfΣ |} ;
-     wf_env_map := Σ.(trans_env_map);
-     wf_env_map_repr := Σ.(trans_env_repr);
- |}.
+#[local] Existing Instance extraction_checker_flags.
 
-Import EGlobalEnv.
+Import EWcbvEval.
 
-Definition eprogram := 
-  (EAst.global_context * EAst.term).
-
-Import EEnvMap.GlobalContextMap (make, global_decls).
-
-Arguments EWcbvEval.eval {wfl} _ _ _.
-
-Definition closed_eprogram (p : eprogram) := 
-  closed_env p.1 && ELiftSubst.closedn 0 p.2.
-
-Definition eval_eprogram (wfl : EWcbvEval.WcbvFlags) (p : eprogram) (t : EAst.term) := 
-  EWcbvEval.eval (wfl:=wfl) p.1 p.2 t.
-
-Definition eprogram_env := 
-  (EEnvMap.GlobalContextMap.t * EAst.term).
-
-Definition closed_eprogram_env (p : eprogram_env) := 
-  let Σ := p.1.(global_decls) in
-  closed_env Σ && ELiftSubst.closedn 0 p.2.
-
-Definition eval_eprogram_env (wfl : EWcbvEval.WcbvFlags) (p : eprogram_env) (t : EAst.term) := 
-  EWcbvEval.eval (wfl:=wfl) p.1.(global_decls) p.2 t.
-
-Lemma wf_glob_fresh Σ : wf_glob Σ -> EnvMap.EnvMap.fresh_globals Σ.
-Proof.
-  induction Σ. constructor; auto.
-  intros wf; depelim wf. constructor; auto.
-Qed.
-  
-Program Definition erase_pcuic_program (p : pcuic_program) 
-  (wfΣ : ∥ wf_ext (H := config.extraction_checker_flags) p.1 ∥)
-  (wt : ∥ ∑ T, typing (H := config.extraction_checker_flags) p.1 [] p.2 T ∥) : eprogram_env :=
-  let wfe := build_wf_env_from_env p.1.1 (map_squash (wf_ext_wf _) wfΣ) in
-  let wfe' := ErasureFunction.make_wf_env_ext wfe p.1.2 wfΣ in
-  let t := ErasureFunction.erase wfe' nil p.2 _ in
-  let Σ' := ErasureFunction.erase_global (EAstUtils.term_global_deps t) wfe in
-  (EEnvMap.GlobalContextMap.make Σ' _, t).
-  
-Next Obligation.
-  sq. destruct wt as [T Ht].
-  cbn in *. subst. now exists T.
-Qed.
-Next Obligation.
-  unfold ErasureFunction.erase_global.
-  eapply wf_glob_fresh.
-  eapply ERemoveParams.erase_global_decls_wf_glob.
-Qed.
-
-
-(* * The full correctness lemma of erasure from Template programs do λ-box
-
-Lemma erase_template_program_correctness {p : Ast.Env.program} univs
-  (Σ := (p.1, univs))
-  {wfΣ : ∥ Typing.wf_ext Σ ∥}
-  {wt : ∥ ∑ T, Typing.typing (p.1, univs) [] p.2 T ∥} {Σ' t'} :
-  erase_template_program p univs wfΣ wt = (Σ', t') ->
-  forall v, WcbvEval.eval p.1 p.2 v ->
-  exists v',
-    PCUICExpandLets.trans_global (trans_global Σ) ;;; [] |- 
-      PCUICExpandLets.trans (trans (trans_global Σ) v) ⇝ℇ v' /\ 
-    ∥ EWcbvEval.eval (wfl:=EWcbvEval.default_wcbv_flags) Σ' t' v' ∥.
-Proof.
-  unfold erase_template_program.
-  intros [= <- <-] v ev.
-  set (expΣ := (PCUICExpandLets.trans_global (trans_global Σ))).
-  set (wfexpΣ := build_wf_env _ _).
-  pose proof (erase_correct wfexpΣ).
-  set (wfexpΣ' := make_wf_env_ext _ _ _) in *.
-  set wftΣ : ∥ wf_ext (PCUICExpandLets.trans_global (trans_global Σ)) ∥ :=
-    wfexpΣ'.(wf_env_ext_wf).
-  specialize (H univs wftΣ (PCUICExpandLets.trans (trans (trans_global Σ) p.2)) (PCUICExpandLets.trans (trans (trans_global Σ) v))).
-  set wtp : PCUICSafeLemmata.welltyped (PCUICExpandLets.trans_global (trans_global Σ)) [] 
-    (PCUICExpandLets.trans (trans (trans_global Σ) p.2)) :=
-    (erase_template_program_obligation_1 p univs wfΣ wt).
-  set (t' := erase wfexpΣ' [] (PCUICExpandLets.trans (trans (trans_global_env p.1) p.2)) wtp) in *.
-  set (deps := (term_global_deps _)).
-  (* change (empty_ext (PCUICExpandLets.trans_global_env (trans_global_env p.1))) with *)
-    (* (PCUICExpandLets.trans_global (trans_global Σ)) in *. *)
-  specialize (H (erase_global deps wfexpΣ)).
-  specialize (H _ deps wtp eq_refl).
-  forward H. eapply Kernames.KernameSet.subset_spec. reflexivity.
-  specialize (H eq_refl).
-  destruct wt, wfΣ.
-  have wfmid : wf (trans_global (p.1, univs)).1.
-  { now eapply template_to_pcuic_env. }
-  forward H.
-  { unfold wfexpΣ. simpl.
-    unshelve eapply (PCUICExpandLetsCorrectness.trans_wcbveval (Σ := (trans_global_env p.1, univs))).
-    { destruct s as [T HT].
-      eapply (PCUICClosedTyp.subject_closed (Γ := [])). 
-      apply (template_to_pcuic_typing (Σ := (p.1, univs)) [] _ T);simpl; eauto.
-      eapply w. Unshelve. now eapply template_to_pcuic_env. }
-    unshelve eapply trans_wcbvEval; eauto. apply w.
-    destruct s as [T HT]. eauto.
-    clear -w HT. now eapply TypingWf.typing_wf in HT. }  
-  destruct H as [v' [Hv He]].
-  sq.
-  set (eΣ := erase_global _ _) in *. exists v'. split => //.
-Qed. *)
-
-Obligation Tactic := idtac.
-
-Import Extract.
-
-Definition expanded_eprogram (p : eprogram_env) := 
-  let decls := p.1.(EEnvMap.GlobalContextMap.global_decls) in
-  EEtaExpandedFix.isEtaExp_env decls && EEtaExpandedFix.isEtaExp decls [] p.2.
-
-Definition expanded_eprogram_cstrs (p : eprogram_env) := 
-  let decls := p.1.(EEnvMap.GlobalContextMap.global_decls) in
-  EEtaExpanded.isEtaExp_env decls && EEtaExpanded.isEtaExp decls p.2.
-  
-Definition erase_program (p : pcuic_program) (wtp : ∥ wt_pcuic_program (cf:=config.extraction_checker_flags) p ∥) : eprogram_env :=
-  erase_pcuic_program p (map_squash fst wtp) (map_squash snd wtp).
-
-Module EtaExpE.
-  Import EAst ErasureFunction EEtaExpandedFix EDeps.
-
-  Definition expanded_constant_decl Σ (cb : constant_body) : Prop :=
-    on_Some_or_None (expanded Σ []) cb.(cst_body).
-      
-  Definition expanded_decl Σ d :=
-    match d with
-    | ConstantDecl cb => expanded_constant_decl Σ cb
-    | InductiveDecl idecl => True
-    end.
-      
-  Inductive expanded_global_declarations : forall (Σ : global_declarations), Prop :=
-  | expanded_global_nil : expanded_global_declarations []
-  | expanded_global_cons decl Σ : expanded_global_declarations Σ -> 
-    expanded_decl Σ decl.2 -> expanded_global_declarations (decl :: Σ).
-
-  Definition expanded_global_env := expanded_global_declarations.
-
-  Definition global_subset (Σ Σ' : global_declarations) := 
-    forall kn d, lookup_env Σ kn = Some d -> lookup_env Σ' kn = Some d.
-  
-  Lemma lookup_env_In d Σ : 
-    wf_glob Σ ->
-    lookup_env Σ d.1 = Some d.2 <-> In d Σ.
-  Proof.
-    intros wf.
-    split.
-    - induction Σ; cbn => //.
-      destruct (eqb_spec d.1 a.1). intros [=]. destruct a, d; cbn in *; intuition auto.
-      left; subst; auto. depelim wf.
-      intros hl; specialize (IHΣ wf hl); intuition auto.
-    - induction wf => /= //.
-      intros [eq|hin]; eauto. subst d.
-      now rewrite eqb_refl.
-      specialize (IHwf hin).
-      destruct (eqb_spec d.1 kn). subst kn.
-      eapply EExtends.lookup_env_Some_fresh in IHwf. contradiction.
-      exact IHwf.
-  Qed.
-
-  Lemma global_subset_In Σ Σ' : 
-    wf_glob Σ -> wf_glob Σ' ->
-    global_subset Σ Σ' <-> forall d, In d Σ -> In d Σ'.
-  Proof.
-    split.
-    - intros g d hin.
-      specialize (g d.1 d.2).
-      eapply lookup_env_In => //.
-      apply g. apply lookup_env_In => //.
-    - intros hd kn d hl.
-      eapply (lookup_env_In (kn, d)) in hl => //.
-      eapply (lookup_env_In (kn, d)) => //. eauto.
-  Qed.
-
-  Lemma global_subset_cons d Σ Σ' : 
-    global_subset Σ Σ' ->
-    global_subset (d :: Σ) (d :: Σ').
-  Proof.
-    intros sub kn d'.
-    cbn. case: eqb_spec => [eq|neq] => //.
-    eapply sub.
-  Qed.
-
-  Lemma fresh_global_subset Σ Σ' kn : 
-    wf_glob Σ -> wf_glob Σ' ->
-    global_subset Σ Σ' ->
-    fresh_global kn Σ' -> fresh_global kn Σ.
-  Proof.
-    intros wfΣ wfΣ' sub fr.
-    unfold fresh_global in *.
-    eapply All_Forall, In_All.
-    intros [kn' d] hin. cbn.
-    intros eq; subst.
-    eapply global_subset_In in hin; tea.
-    eapply Forall_All in fr. eapply All_In in fr; tea.
-    destruct fr. cbn in H. congruence.
-  Qed.
-
-  Lemma global_subset_cons_right d Σ Σ' : 
-    wf_glob Σ -> wf_glob (d :: Σ') ->
-    global_subset Σ Σ' ->
-    global_subset Σ (d :: Σ').
-  Proof.
-    intros wf wf' gs.
-    assert (wf_glob Σ'). now depelim wf'.
-    rewrite (global_subset_In _ _ wf H) in gs.
-    rewrite global_subset_In //.
-    intros decl. specialize (gs decl).
-    intros hin; specialize (gs hin). cbn. now right.
-  Qed.
-    
-  Lemma lookup_erase_global (cf := config.extraction_checker_flags) {Σ : wf_env} {deps deps'} :
-    KernameSet.Subset deps deps' ->
-    global_subset (erase_global deps Σ) (erase_global deps' Σ).
-  Proof.
-    unfold erase_global.
-    destruct Σ as [[[univs Σ] wfΣ G wfG] map repr]. cbn in *. clear G wfG.
-    revert deps deps' wfΣ map repr.
-    induction Σ. cbn => //.
-    intros deps deps' wfΣ map repr sub.
-    destruct a as [kn' []]; cbn;
-    (set (decl := E.ConstantDecl _) || set (decl := E.InductiveDecl _)); hidebody decl;
-    set (eg := erase_global_decls _ _ _ _); hidebody eg;
-    set (eg' := erase_global_decls _ _ _ _); hidebody eg';
-    try (set (eg'' := erase_global_decls _ _ _ _); hidebody eg'');
-    try (set (eg''' := erase_global_decls _ _ _ _); hidebody eg''').
-    { destruct (KernameSet.mem) eqn:knm => /=.
-      + eapply KernameSet.mem_spec, sub, KernameSet.mem_spec in knm. rewrite knm.
-        apply global_subset_cons. eapply IHΣ.
-        intros x hin. eapply KernameSet.union_spec in hin.
-        eapply KernameSet.union_spec. destruct hin. left. now eapply sub.
-        right => //.
-      + destruct (KernameSet.mem kn' deps') eqn:eq'.
-        eapply global_subset_cons_right.
-        eapply ERemoveParams.erase_global_wf_glob.
-        constructor. eapply ERemoveParams.erase_global_wf_glob.
-        eapply ERemoveParams.erase_global_decls_fresh.
-        clear -wfΣ. destruct wfΣ. destruct X as [onu ond]; cbn in *.
-        now depelim ond.
-        eapply IHΣ.
-        intros x hin.
-        eapply KernameSet.union_spec. left. now eapply sub.
-        eapply IHΣ => //. }
-    { destruct (KernameSet.mem) eqn:knm => /=.
-      + eapply KernameSet.mem_spec, sub, KernameSet.mem_spec in knm. rewrite knm.
-        apply global_subset_cons. eapply IHΣ => //.
-      + destruct (KernameSet.mem kn' deps') eqn:eq'.
-        eapply global_subset_cons_right. eapply ERemoveParams.erase_global_wf_glob.
-        constructor. eapply ERemoveParams.erase_global_wf_glob.
-        eapply ERemoveParams.erase_global_decls_fresh.
-        clear -wfΣ. destruct wfΣ. destruct X as [onu ond]; cbn in *. now depelim ond.
-        eapply IHΣ. intros x hin. now eapply sub.
-        eapply IHΣ => //. }
-  Qed.
-  
-  Lemma expanded_weakening_global Σ deps deps' Γ t : 
-    KernameSet.Subset deps deps' ->
-    expanded (erase_global deps Σ) Γ t ->
-    expanded (erase_global deps' Σ) Γ t.
-  Proof.
-    intros hs.
-    eapply expanded_ind; intros; try solve [econstructor; eauto].
-    eapply expanded_tConstruct_app; tea.
-    destruct H. split; tea.
-    destruct d; split => //.
-    cbn in *. red in H.
-    eapply lookup_erase_global in H; tea.
-  Qed.
-
-  Lemma expanded_erase (cf := config.extraction_checker_flags) {Σ : wf_env} univs wfΣ t wtp :
-    PCUICEtaExpand.expanded Σ [] t ->
-    let Σ' := make_wf_env_ext Σ univs wfΣ in
-    let et := (erase Σ' [] t wtp) in
-    let deps := EAstUtils.term_global_deps et in
-    EEtaExpandedFix.expanded (erase_global deps Σ) [] et.
-  Proof.
-    intros hexp Σ'.
-    have [wf] : ∥ wf Σ ∥.
-    { destruct wfΣ. sq. exact w. }
-    eapply (expanded_erases (Σ := (Σ, univs))); tea.
-    eapply (erases_erase (Σ := Σ')). cbn.
-    eapply (erases_deps_erase (Σ := Σ) univs wfΣ).
-  Qed.
-
-  Lemma expanded_erase_global (cf := config.extraction_checker_flags) deps {Σ: wf_env} :
-    EtaExpPCUIC.expanded_global_env Σ ->
-    expanded_global_env (erase_global deps Σ).
-  Proof.
-    intros etaΣ.
-    unfold erase_global.
-    destruct Σ as [Σ map repr]. cbn in *.
-    destruct Σ as [Σ wfΣ G isG]. cbn in *. clear G isG.
-    destruct Σ as [univs Σ]; cbn in *.
-    red. revert wfΣ. red in etaΣ. cbn in *.
-    revert deps map repr.
-    induction etaΣ; intros deps. cbn. constructor.
-    destruct decl as [kn []];
-    destruct (KernameSet.mem kn deps) eqn:eqkn; simpl; rewrite eqkn.
-    constructor; [eapply IHetaΣ; auto|].
-    red. cbn. red. cbn in *.
-    set (deps' := KernameSet.union _ _). hidebody deps'.
-    set (wfext := make_wf_env_ext _ _ _). hidebody wfext.
-    destruct H.
-    destruct c as [cst_na [cst_body|] cst_type cst_rel].
-    cbn in *.
-    eapply expanded_weakening_global. 
-    2:{ eapply expanded_erase; tea. }
-    set (et := erase _ _ _ _) in *.
-    unfold deps'. unfold hidebody. intros x hin.    
-    eapply KernameSet.union_spec. right => //.
-    now cbn.
-    intros.
-    eapply IHetaΣ.
-    intros map repr wfΣ.
-    constructor. eapply IHetaΣ.
-    red. cbn => //.
-    intros map repr wfΣ.
-    eapply IHetaΣ.
-  Qed.
-  
-  Lemma expanded_global_env_isEtaExp_env {Σ} : expanded_global_env Σ -> isEtaExp_env Σ.
-  Proof.
-    intros e; induction e; cbn => //.
-    rewrite IHe andb_true_r.
-    red in H; red. destruct decl as [kn []] => /= //.
-    cbn in H. red in H. unfold isEtaExp_constant_decl.
-    destruct (cst_body c); cbn in * => //.
-    now eapply expanded_isEtaExp.
-  Qed.
-
-  Ltac simp_eta := simp isEtaExp; rewrite -?isEtaExp_equation_1 -?EEtaExpanded.isEtaExp_equation_1.
-
-  Lemma isEtaExpFix_isEtaExp Σ Γ t : isEtaExp Σ Γ t -> EEtaExpanded.isEtaExp Σ t.
-  Proof.
-    funelim (isEtaExp Σ Γ t); try solve [simp_eta => //].
-    - simp_eta in Heqcall. simp_eta.
-      intros Ha. eapply In_All in H. solve_all.
-    - simp_eta. rtoProp; intuition auto.
-    - simp_eta. rtoProp; intuition auto.
-      eapply In_All in H0; solve_all.
-    - eapply In_All in H. simp_eta; rtoProp; intuition auto. solve_all.
-    - eapply In_All in H. simp_eta; rtoProp; intuition auto.
-      move: H0; rewrite isEtaExp_mkApps // /=.
-      move=> /andP[] etaind etav.
-      rewrite EEtaExpanded.isEtaExp_Constructor. apply/andP; split. exact etaind.
-      solve_all.
-    - eapply In_All in H, H0. simp_eta in Heqcall.
-      clear Heqcall.
-      rewrite isEtaExp_mkApps // /= => /andP[] /andP[] etafix etamfix etav.
-      eapply EEtaExpanded.isEtaExp_mkApps_intro. simp_eta.
-      clear -H etamfix. solve_all.
-      solve_all.
-    - eapply In_All in H. clear Heqcall.
-      rewrite isEtaExp_mkApps // /= => /andP[] etarel etav.
-      eapply EEtaExpanded.isEtaExp_mkApps_intro. simp_eta. solve_all.
-    - eapply In_All in H0. clear Heqcall.
-      rewrite isEtaExp_mkApps // /= Heq => /andP[] etau etav.
-      eapply EEtaExpanded.isEtaExp_mkApps_intro; auto. solve_all.
-  Qed.
-
-  Lemma isEtaExpFix_env_isEtaExp_env Σ : isEtaExp_env Σ -> EEtaExpanded.isEtaExp_env Σ.
-  Proof.
-    induction Σ; cbn; auto.
-    move/andP => [] etaa etaΣ.
-    rewrite IHΣ // andb_true_r.
-    move: etaa. rewrite /isEtaExp_decl /EEtaExpanded.isEtaExp_decl.
-    destruct a.2 => //.
-    rewrite /isEtaExp_constant_decl /EEtaExpanded.isEtaExp_constant_decl.
-    destruct (E.cst_body c) => // /=.
-    eapply isEtaExpFix_isEtaExp.
-  Qed.
-
-  Lemma expanded_erase_program (cf := config.extraction_checker_flags) p (wtp : ∥ wt_pcuic_program p ∥) :
-    EtaExpPCUIC.expanded_pcuic_program p ->
-    expanded_eprogram (erase_program p wtp).
-  Proof.
-    intros [etaenv etat]. apply /andP; split.
-    eapply expanded_global_env_isEtaExp_env, expanded_erase_global, etaenv.
-    eapply expanded_isEtaExp, expanded_erase, etat.
-  Qed.
-
-End EtaExpE.
-
-Program Definition erase_transform : Transform.t pcuic_program eprogram_env term EAst.term eval_pcuic_program (eval_eprogram_env EWcbvEval.default_wcbv_flags) :=
- {| name := "erasure";
-    pre p :=  
-      ∥ wt_pcuic_program (cf := config.extraction_checker_flags) p ∥ /\ EtaExpPCUIC.expanded_pcuic_program p ;
-    transform p hp := erase_program p (proj1 hp) ;
-    post p :=
-      let decls := p.1.(global_decls) in
-      [/\ wf_glob decls, closed_eprogram_env p & expanded_eprogram p];
-    obseq g g' v v' := let Σ := g.1 in Σ ;;; [] |- v ⇝ℇ v' |}.
-Next Obligation.
-  cbn -[erase_program].
-  intros p [wtp etap].
-  destruct erase_program eqn:e.
-  split; cbn.
-  - unfold erase_program, erase_pcuic_program in e. simpl. injection e. intros <- <-. 
-    eapply ERemoveParams.erase_global_wf_glob.
-  - apply/andP; split.
-    * unfold erase_program, erase_pcuic_program in e. simpl. injection e. intros <- <-. 
-      eapply ErasureFunction.erase_global_closed.
-    * unfold erase_program, erase_pcuic_program in e. simpl. injection e. intros <- <-. 
-      eapply (ErasureFunction.erases_closed _ []). eapply ErasureFunction.erases_erase.
-      clear e. destruct wtp as [[wfΣ [T HT]]].
-      now eapply (@PCUICClosedTyp.subject_closed _ _) in HT.
-  - rewrite -e. cbn.
-    now eapply EtaExpE.expanded_erase_program.
-Qed.
-
-Next Obligation.
-  red. move=> [Σ t] v [[wf [T HT]]]. unfold eval_pcuic_program, eval_eprogram.
-  intros ev.
-  destruct erase_program eqn:e.
-  unfold erase_program, erase_pcuic_program in e. simpl in e. injection e; intros <- <-.
-  simpl. clear e. cbn in *.
-  set (Σ' := build_wf_env_from_env _ _).
-  eapply (ErasureFunction.erase_correct Σ' Σ.2 _ _ _ _ _ (EAstUtils.term_global_deps _)) in ev; try reflexivity.
-  2:eapply Kernames.KernameSet.subset_spec; reflexivity.
-  destruct ev as [v' [he [hev]]]. exists v'; split; split => //.
-  red. cbn.
-  eexact hev.
-Qed.
-
-Import EOptimizePropDiscr.
-
-Program Definition optimize_prop_discr_optimization : self_transform eprogram EAst.term (eval_eprogram EWcbvEval.default_wcbv_flags) (eval_eprogram EWcbvEval.opt_wcbv_flags) := 
-  {| name := "optimize_prop_discr"; 
-    transform p _ := 
-      (EOptimizePropDiscr.optimize_env p.1, EOptimizePropDiscr.optimize p.1 p.2);
-    pre := closed_eprogram;
-    post := closed_eprogram;
-    obseq g g' v v' := v' = EOptimizePropDiscr.optimize g.1 v
-    |}.
-
-Next Obligation.
-  move=> [Σ t] /andP[cle clt].
-  cbn in *. apply/andP; split.
-  move: cle. cbn. induction Σ at 1 3; cbn; auto.
-  move/andP => [] cla clg. rewrite (IHg clg) andb_true_r.
-  destruct a as [kn []]; cbn in * => //.
-  destruct Extract.E.cst_body => //. cbn in cla |- *.
-  now eapply EOptimizePropDiscr.closed_optimize.
-  now eapply EOptimizePropDiscr.closed_optimize.
-Qed.
-Next Obligation.
-  red. move=> [Σ t] /= v /andP[cle clt] ev.
-  eapply EOptimizePropDiscr.optimize_correct in ev; eauto.
-Qed.
-
-Program Definition remove_params (p : eprogram_env) : eprogram :=
-  (ERemoveParams.strip_env p.1, ERemoveParams.strip p.1 p.2).
-
-Program Definition remove_params_optimization (fl : EWcbvEval.WcbvFlags) : 
-  Transform.t eprogram_env eprogram EAst.term EAst.term (eval_eprogram_env fl) (eval_eprogram fl) :=
-  {| name := "remove_parameters";
-    transform p pre := remove_params p;
-    pre p := 
-    let decls := p.1.(global_decls) in
-     [/\ wf_glob decls, closed_eprogram_env p & expanded_eprogram_cstrs p ];
-    post := closed_eprogram;
-    obseq g g' v v' := v' = (ERemoveParams.strip g.1 v) |}.
-Next Obligation.
-  move=> fl [Σ t] [wfe /andP[cle clt] etap].
-  simpl.
-  cbn -[ERemoveParams.strip] in *.
-  apply/andP; split; cbn.
-  move: cle. unfold closed_env. unfold ERemoveParams.strip_env.
-  rewrite forallb_map. eapply forallb_impl. intros.
-  destruct x as [kn []]; cbn in * => //.
-  destruct Extract.E.cst_body => //. cbn -[ERemoveParams.strip] in H0 |- *.
-  now eapply ERemoveParams.closed_strip.
-  now eapply ERemoveParams.closed_strip.
-Qed.
-
-Next Obligation.
-  red. move=> ? [Σ t] /= v [wfe /andP[cle clt] etap] ev.
-  eapply ERemoveParams.strip_eval in ev; eauto.
-  all:move/andP: etap => [] => //.
-Qed.
-
-Program Definition remove_params_fast_optimization (fl : EWcbvEval.WcbvFlags) :
-  Transform.t eprogram_env eprogram EAst.term EAst.term (eval_eprogram_env fl) (eval_eprogram fl) :=
-  {| name := "remove_parameters_fast";
-    transform p _ := (ERemoveParams.Fast.strip_env p.1, ERemoveParams.Fast.strip p.1 [] p.2);
-    pre p := 
-      let decls := p.1.(global_decls) in
-      [/\ wf_glob decls, closed_eprogram_env p & expanded_eprogram_cstrs p];
-    post := closed_eprogram;
-    obseq g g' v v' := v' = (ERemoveParams.strip g.1 v) |}.
-Next Obligation.
-  move=> fl [Σ t] [wfe /andP[cle clt] etap].
-  simpl.
-  apply/andP.
-  rewrite -ERemoveParams.Fast.strip_fast -ERemoveParams.Fast.strip_env_fast.
-  cbn -[ERemoveParams.strip] in *.
-  split.
-  move: cle. unfold closed_env. unfold ERemoveParams.strip_env.
-  rewrite forallb_map. eapply forallb_impl. intros.
-  destruct x as [kn []]; cbn in * => //.
-  destruct Extract.E.cst_body => //. cbn -[ERemoveParams.strip] in H0 |- *.
-  now eapply ERemoveParams.closed_strip.
-  now eapply ERemoveParams.closed_strip.
-Qed.
-Next Obligation.
-  red. move=> ? [Σ t] /= v [wfe /andP[cle clt] etap] ev.
-  rewrite -ERemoveParams.Fast.strip_fast -ERemoveParams.Fast.strip_env_fast.
-  eapply ERemoveParams.strip_eval in ev; eauto.
-  all:move/andP: etap => [] => //.
-Qed.
-
-Obligation Tactic := program_simpl.
-
-Program Definition erasure_pipeline := 
+Program Definition erasure_pipeline :
+ Transform.t TemplateProgram.template_program EProgram.eprogram 
+  Ast.term EAst.term
+  TemplateProgram.eval_template_program
+  (EProgram.eval_eprogram {| with_prop_case := false; with_guarded_fix := false |}) := 
+  (* Eta expansion of constructors and fixpoints *)
   template_eta_expand ▷
+  (* Casts are removed, application is binary, case annotations are inferred from the global environment *)
   template_to_pcuic_transform ▷
+  (* Branches of cases are expanded to bind only variables, constructor types are expanded accordingly *)
   pcuic_expand_lets_transform ▷
-  erase_transform ▷ 
-  remove_params_optimization _ ▷ 
+  (* Erasure of proofs terms in Prop and types *)
+  erase_transform ▷
+  (* Simulation of the guarded fixpoint rules with a single unguarded one: the only "stuck" fixpoints 
+     remaining are unapplied.  *)
+  guarded_to_unguarded_fix eq_refl ▷
+  (* Remove all constructor parameters *)
+  remove_params_optimization ▷ 
+  (* Remove all cases of propositional content *)
   optimize_prop_discr_optimization.
 
-Lemma expanded_eprogram_expanded_eprogram_cstrs p : 
-  expanded_eprogram p ->
-  expanded_eprogram_cstrs p.
-Proof.
-  move=> /andP[] etaenv etat.
-  apply /andP. split; [now eapply EtaExpE.isEtaExpFix_env_isEtaExp_env|
-  now eapply EtaExpE.isEtaExpFix_isEtaExp].
+Next Obligation.
+  destruct H. split => //. sq.
+  now eapply EProgram.expanded_eprogram_expanded_eprogram_cstrs. 
 Qed.
 
-Next Obligation.
-  destruct H. split => //. now eapply expanded_eprogram_expanded_eprogram_cstrs. 
-Qed.
+(* For now we only give out that erased programs are closed, but 
+  they are also eta-expanded and well-scoped w.r.t. the global environment *)
+Eval simpl in post (guarded_to_unguarded_fix _).
 
 Definition run_erase_program := run erasure_pipeline.
 
 Program Definition erasure_pipeline_fast := 
+  template_eta_expand ▷
   template_to_pcuic_transform ▷
   pcuic_expand_lets_transform ▷
   erase_transform ▷ 
   remove_params_fast_optimization _ ▷ 
   optimize_prop_discr_optimization.
 Next Obligation.
-  destruct H; split => //. now eapply expanded_eprogram_expanded_eprogram_cstrs. 
+  destruct H; split => //. now eapply EProgram.expanded_eprogram_expanded_eprogram_cstrs. 
 Qed.
 
 Definition run_erase_program_fast := run erasure_pipeline_fast.
@@ -591,8 +79,11 @@ Local Open Scope string_scope.
   Coq definition). *)
 Program Definition erase_and_print_template_program {cf : checker_flags} (p : Ast.Env.program)
   : string :=
-  let p' := run_erase_program p (todo "wf_env and welltyped term") in
+  let p' := run_erase_program p _ in
   time "Pretty printing" EPretty.print_program p'.
+Next Obligation.
+  sq. red. todo "assuming quoted environment and term are wellformed".
+Qed.
 
 Program Definition erase_fast_and_print_template_program {cf : checker_flags} (p : Ast.Env.program)
   : string :=
