pcuic/theories/PCUICProgram.v
@@ -1,118 +1,49 @@
 (** * Definition of programs in template-coq, well-typed terms and provided transformations **)
 From Coq Require Import ssreflect.
-From MetaCoq.Template Require Import
-        utils
-        Ast           (* The term AST *)
-        Typing        (* Typing judgment *)
-        config        (* Typing configuration *)
-        Transform        
-        TemplateProgram.
+From MetaCoq.Template Require Import utils config EnvMap.
+From MetaCoq.PCUIC Require Import PCUICAstUtils PCUICAst PCUICGlobalEnv PCUICTyping.
 
-From MetaCoq.PCUIC Require Import PCUICAstUtils PCUICAst TemplateToPCUIC
-    TemplateToPCUICWcbvEval
-    TemplateToPCUICCorrectness 
-    TemplateToPCUICExpanded
-    PCUICGlobalEnv PCUICTyping PCUICEtaExpand.
+(** Global environment with a map for efficient lookups *)
 
-Import Transform.
-
-(** * Translation from Template to PCUIC, directly preserves evaluation *)
-
-Definition eval_pcuic_program (p : pcuic_program) (v : term) :=
-  ∥ PCUICWcbvEval.eval p.1.(trans_env_env) p.2 v ∥.
-      
-Definition template_to_pcuic_obseq (p : Ast.Env.program) (p' : pcuic_program) (v : Ast.term) (v' : term) :=
-  let Σ := Ast.Env.empty_ext p.1 in v' = trans (trans_global Σ) v.
-
-Lemma trans_template_program_wt {cf : checker_flags} p (wtp : wt_template_program p) : wt_pcuic_program (trans_template_program p).
-Proof.
-  move: p wtp.
-  intros [Σ t] [wfext ht].
-  unfold wt_pcuic_program, trans_template_program; cbn in *.
-  cbn. split. eapply template_to_pcuic_env_ext in wfext. apply wfext.
-  destruct ht as [T HT]. exists (trans (trans_global_env Σ) T).
-  eapply (template_to_pcuic_typing (Σ := Ast.Env.empty_ext Σ) []). apply wfext.
-  apply HT.
-Qed.
-
-Program Definition template_to_pcuic_transform {cf : checker_flags} : 
-  Transform.t template_program pcuic_program Ast.term term 
-  eval_template_program eval_pcuic_program :=
- {| name := "template to pcuic";
-    pre p := ∥ wt_template_program p ∥ /\ EtaExpand.expanded_program p ;
-    transform p _ := trans_template_program p ;
-    post p := ∥ wt_pcuic_program p ∥ /\ PCUICEtaExpand.expanded_pcuic_program p;
-    obseq := template_to_pcuic_obseq |}.
-Next Obligation.
-  cbn. intros cf p [[wtp] etap].
-  split; [split|].
-  now eapply trans_template_program_wt.
-  now eapply expanded_trans_program in etap.
-Qed.
-Next Obligation.
-  red. intros cf [Σ t] v [[]].
-  unfold eval_pcuic_program, eval_template_program.
-  cbn. intros [ev].
-  unshelve eapply TemplateToPCUICWcbvEval.trans_wcbvEval in ev; eauto. apply X.
-  eexists; split; split; eauto.
-  eapply template_to_pcuic_env.
-  apply X. destruct X as [wfΣ [T HT]]. apply TypingWf.typing_wf in HT. apply HT. auto.
-Qed.
-
-From MetaCoq.PCUIC Require Import PCUICExpandLets PCUICExpandLetsCorrectness.
-
-(** Expansion of let bindings in constructor types / case branches. 
-    Direcly preserves evaluation as well: the new value is simply the 
-    expansion of the old one, which is the identiy on normal forms.
-*)
+Record global_env_map := 
+  { trans_env_env :> global_env;
+    trans_env_map : EnvMap.t global_decl; 
+    trans_env_repr : EnvMap.repr trans_env_env.(declarations) trans_env_map }.
 
 Program Definition build_global_env_map (g : global_env) : global_env_map := 
   {| trans_env_env := g; 
      trans_env_map := EnvMap.EnvMap.of_global_env g.(declarations) |}.
-Next Obligation.
-  intros g. eapply EnvMap.EnvMap.repr_global_env.
-Qed.
+  
+Definition global_env_ext_map := global_env_map * universes_decl.
 
-Definition let_expansion_obseq (p : pcuic_program) (p' : pcuic_program) (v : term) (v' : term) :=
-  v' = PCUICExpandLets.trans v.
+Definition pcuic_program : Type := global_env_ext_map * term.
+  
+Definition global_env_ext_map_global_env_ext (g : global_env_ext_map) : global_env_ext :=
+  (trans_env_env (fst g), g.2).
+Coercion global_env_ext_map_global_env_ext : global_env_ext_map >-> global_env_ext.
 
-Definition expand_lets_program (p : pcuic_program) : pcuic_program :=
-  let Σ' := PCUICExpandLets.trans_global p.1 in 
-  ((build_global_env_map Σ', p.1.2), PCUICExpandLets.trans p.2).
-    
-Lemma expanded_expand_lets_program {cf : checker_flags} p (wtp : wt_pcuic_program p) :
-  expanded_pcuic_program p ->
-  expanded_pcuic_program (expand_lets_program p).
-Proof.
-  destruct p as [[Σ udecl] t]; intros [etaenv etat].
-  destruct wtp as [wfΣ wtp].
-  cbn in *. split; cbn.
-  now eapply (expanded_global_env_expand_lets (cf:=cf) (Σ, udecl)). 
-  cbn in *.
-  now eapply expanded_expand_lets in etat.
-Qed.
+Definition global_env_ext_map_global_env_map : global_env_ext_map -> global_env_map := fst.
+Coercion global_env_ext_map_global_env_map : global_env_ext_map >-> global_env_map.
 
-Program Definition pcuic_expand_lets_transform {cf : checker_flags} : 
-  self_transform pcuic_program term eval_pcuic_program eval_pcuic_program :=
- {| name := "let expansion in branches/constructors";
-    pre p := ∥ wt_pcuic_program p ∥ /\ PCUICEtaExpand.expanded_pcuic_program p ;
-    transform p hp := expand_lets_program p;
-    post p := ∥ wt_pcuic_program (cf:=PCUICExpandLetsCorrectness.cf' cf) p ∥ /\ PCUICEtaExpand.expanded_pcuic_program p;
-    obseq := let_expansion_obseq |}.
-Next Obligation.
-  intros cf [Σ t] [[[wfext ht]] etap].
-  cbn. split. sq. unfold build_global_env_map. unfold global_env_ext_map_global_env_ext. simpl.
-  split. eapply PCUICExpandLetsCorrectness.trans_wf_ext in wfext. apply wfext.
-  destruct ht as [T HT]. exists (PCUICExpandLets.trans T).
-  eapply (PCUICExpandLetsCorrectness.pcuic_expand_lets Σ []) => //.
-  apply wfext. apply PCUICExpandLetsCorrectness.trans_wf_ext in wfext. apply wfext.
-  now eapply expanded_expand_lets_program.
-Qed.
-Next Obligation.
-  red. intros cf [Σ t] v [[]].
-  unfold eval_pcuic_program.
-  cbn. intros [ev]. destruct X.
-  eapply (PCUICExpandLetsCorrectness.trans_wcbveval (Σ:=global_env_ext_map_global_env_ext Σ)) in ev.
-  eexists; split; split; eauto.
-  destruct s as [T HT]. now apply PCUICClosedTyp.subject_closed in HT.
-Qed.
+(* A well-typed PCUIC program consists of a well-formed environment and term *)
+
+Definition wt_pcuic_program {cf : checker_flags} (p : pcuic_program) :=
+  wf_ext p.1 × ∑ T, typing p.1 [] p.2 T.
+
+Module TransLookup.
+  Definition lookup_minductive (Σ : global_env_map) mind :=
+    match EnvMap.lookup mind Σ.(trans_env_map) with
+    | Some (InductiveDecl decl) => Some decl
+    | _ => None
+    end.
+
+  Definition lookup_inductive Σ ind :=
+    match lookup_minductive Σ (inductive_mind ind) with
+    | Some mdecl => 
+      match nth_error mdecl.(ind_bodies) (inductive_ind ind) with
+      | Some idecl => Some (mdecl, idecl)
+      | None => None
+      end
+    | None => None
+    end.
+End TransLookup.
