erasure/theories/ETransform.v
@@ -1,0 +1,174 @@
+(* Distributed under the terms of the MIT license. *)
+From Coq Require Import Program ssreflect ssrbool.
+From Equations Require Import Equations.
+From MetaCoq.Template Require Import Transform bytestring config utils BasicAst uGraph.
+From MetaCoq.Template Require Pretty Environment Typing WcbvEval EtaExpand.
+Set Warnings "-notation-overridden".
+From MetaCoq.PCUIC Require PCUICAst PCUICAstUtils PCUICProgram PCUICTransform.
+Set Warnings "+notation-overridden".
+From MetaCoq.SafeChecker Require Import PCUICErrors PCUICWfEnvImpl.
+From MetaCoq.Erasure Require EAstUtils ErasureFunction ErasureCorrectness EPretty Extract EProgram.
+
+Import PCUICAst (term) PCUICProgram PCUICTransform (eval_pcuic_program) Extract EProgram
+    EAst Transform.
+Import EEnvMap EGlobalEnv.
+
+Program Definition erase_transform : Transform.t pcuic_program eprogram_env PCUICAst.term EAst.term 
+  eval_pcuic_program (eval_eprogram_env EWcbvEval.default_wcbv_flags) :=
+ {| name := "erasure";
+    pre p :=  
+      ∥ wt_pcuic_program (cf := config.extraction_checker_flags) p ∥ /\ PCUICEtaExpand.expanded_pcuic_program p ;
+    transform p hp := erase_program p (proj1 hp) ;
+    post p :=
+      let decls := p.1.(GlobalContextMap.global_decls) in
+      [/\ wf_glob decls, closed_eprogram_env p & expanded_eprogram p];
+    obseq g g' v v' := let Σ := g.1 in Σ ;;; [] |- v ⇝ℇ v' |}.
+Next Obligation.
+  cbn -[erase_program].
+  intros p [wtp etap].
+  destruct erase_program eqn:e.
+  split; cbn.
+  - unfold erase_program, erase_pcuic_program in e. simpl. injection e. intros <- <-. 
+    eapply ErasureFunction.erase_global_wf_glob.
+  - apply/andP; split.
+    * unfold erase_program, erase_pcuic_program in e. simpl. injection e. intros <- <-. 
+      eapply ErasureFunction.erase_global_closed.
+    * unfold erase_program, erase_pcuic_program in e. simpl. injection e. intros <- <-. 
+      eapply (ErasureFunction.erases_closed _ []). eapply ErasureFunction.erases_erase.
+      clear e. destruct wtp as [[wfΣ [T HT]]].
+      now eapply (@PCUICClosedTyp.subject_closed _ _) in HT.
+  - rewrite -e. cbn.
+    now eapply expanded_erase_program.
+Qed.
+
+Next Obligation.
+  red. move=> [Σ t] v [[wf [T HT]]]. unfold eval_pcuic_program, eval_eprogram.
+  intros [ev].
+  destruct erase_program eqn:e.
+  unfold erase_program, erase_pcuic_program in e. simpl in e. injection e; intros <- <-.
+  simpl. clear e. cbn in *.
+  set (Σ' := build_wf_env_from_env _ _).
+  eapply (ErasureFunction.erase_correct Σ' Σ.2 _ _ _ _ _ (EAstUtils.term_global_deps _)) in ev; try reflexivity.
+  2:eapply Kernames.KernameSet.subset_spec; reflexivity.
+  destruct ev as [v' [he [hev]]]. exists v'; split => //.
+  red. cbn.
+  sq. eexact hev.
+Qed.
+
+(** This transformation is the identity on terms but changes the evaluation relation to one
+    where fixpoints are not guarded. It requires eta-expanded fixpoints and evaluation 
+    to use the guarded fixpoint rule as a precondition. *)
+
+Import EWcbvEval (WcbvFlags, with_prop_case, with_guarded_fix).
+
+Program Definition guarded_to_unguarded_fix {fl : EWcbvEval.WcbvFlags} (wguard : with_guarded_fix) :
+  Transform.t eprogram_env eprogram_env EAst.term EAst.term 
+    (eval_eprogram_env fl) (eval_eprogram_env (EEtaExpandedFix.switch_unguarded_fix fl)) :=
+  {| name := "switching to unguarded fixpoints";
+    transform p pre := p;
+    pre p := 
+    let decls := p.1.(GlobalContextMap.global_decls) in
+     [/\ wf_glob decls, closed_eprogram_env p & expanded_eprogram p ];
+    post p := let decls := p.1.(GlobalContextMap.global_decls) in
+     [/\ wf_glob decls, closed_eprogram_env p & expanded_eprogram p ];
+    obseq g g' v v' := v' = v |}.
+Next Obligation. cbn. eauto. Qed.
+Next Obligation.
+  cbn.
+  move=> fl wguard [Σ t] v [wfe /andP[cle clt] /andP[etae etat]]. cbn in *.
+  intros [ev]. exists v. split => //.
+  red. sq. cbn in *.
+  now apply EEtaExpandedFix.eval_opt_to_target.
+Qed.
+
+Program Definition remove_params (p : eprogram_env) : eprogram :=
+  (ERemoveParams.strip_env p.1, ERemoveParams.strip p.1 p.2).
+
+Program Definition remove_params_optimization {fl : EWcbvEval.WcbvFlags} : 
+  Transform.t eprogram_env eprogram EAst.term EAst.term (eval_eprogram_env fl) (eval_eprogram fl) :=
+  {| name := "stripping constructor parameters";
+    transform p pre := remove_params p;
+    pre p := 
+    let decls := p.1.(GlobalContextMap.global_decls) in
+     [/\ wf_glob decls, closed_eprogram_env p & expanded_eprogram_cstrs p ];
+    post := closed_eprogram;
+    obseq g g' v v' := v' = (ERemoveParams.strip g.1 v) |}.
+Next Obligation.
+  move=> fl [Σ t] [wfe /andP[cle clt] etap].
+  simpl.
+  cbn -[ERemoveParams.strip] in *.
+  apply/andP; split; cbn.
+  move: cle. unfold closed_env. unfold ERemoveParams.strip_env.
+  rewrite forallb_map. eapply forallb_impl. intros.
+  destruct x as [kn []]; cbn in * => //.
+  destruct Extract.E.cst_body => //. cbn -[ERemoveParams.strip] in H0 |- *.
+  now eapply ERemoveParams.closed_strip.
+  now eapply ERemoveParams.closed_strip.
+Qed.
+
+Next Obligation.
+  red. move=> ? [Σ t] /= v [wfe /andP[cle clt] etap] [ev].
+  eapply ERemoveParams.strip_eval in ev; eauto.
+  eexists; split => //. now sq.
+  all:move/andP: etap => [] => //.
+Qed.
+
+Program Definition remove_params_fast_optimization (fl : EWcbvEval.WcbvFlags) :
+  Transform.t eprogram_env eprogram EAst.term EAst.term (eval_eprogram_env fl) (eval_eprogram fl) :=
+  {| name := "stripping constructor parameters (faster?)";
+    transform p _ := (ERemoveParams.Fast.strip_env p.1, ERemoveParams.Fast.strip p.1 [] p.2);
+    pre p := 
+      let decls := p.1.(GlobalContextMap.global_decls) in
+      [/\ wf_glob decls, closed_eprogram_env p & expanded_eprogram_cstrs p];
+    post := closed_eprogram;
+    obseq g g' v v' := v' = (ERemoveParams.strip g.1 v) |}.
+Next Obligation.
+  move=> fl [Σ t] [wfe /andP[cle clt] etap].
+  simpl.
+  apply/andP.
+  rewrite -ERemoveParams.Fast.strip_fast -ERemoveParams.Fast.strip_env_fast.
+  cbn -[ERemoveParams.strip] in *.
+  split.
+  move: cle. unfold closed_env. unfold ERemoveParams.strip_env.
+  rewrite forallb_map. eapply forallb_impl. intros.
+  destruct x as [kn []]; cbn in * => //.
+  destruct Extract.E.cst_body => //. cbn -[ERemoveParams.strip] in H0 |- *.
+  now eapply ERemoveParams.closed_strip.
+  now eapply ERemoveParams.closed_strip.
+Qed.
+Next Obligation.
+  red. move=> ? [Σ t] /= v [wfe /andP[cle clt] etap] [ev].
+  rewrite -ERemoveParams.Fast.strip_fast -ERemoveParams.Fast.strip_env_fast.
+  eapply ERemoveParams.strip_eval in ev; eauto.
+  eexists; split => //. now sq.
+  all:move/andP: etap => [] => //.
+Qed.
+
+Import EOptimizePropDiscr EWcbvEval.
+
+Program Definition optimize_prop_discr_optimization {fl : WcbvFlags} : 
+  self_transform eprogram EAst.term (eval_eprogram fl) 
+    (eval_eprogram (disable_prop_cases fl)) := 
+  {| name := "optimize_prop_discr"; 
+    transform p _ := 
+      (EOptimizePropDiscr.optimize_env p.1, EOptimizePropDiscr.optimize p.1 p.2);
+    pre := closed_eprogram;
+    post := closed_eprogram;
+    obseq g g' v v' := v' = EOptimizePropDiscr.optimize g.1 v
+    |}.
+
+Next Obligation.
+  move=> fl [Σ t] /andP[cle clt].
+  cbn in *. apply/andP; split.
+  move: cle. cbn. induction Σ at 1 3; cbn; auto.
+  move/andP => [] cla clg. rewrite (IHg clg) andb_true_r.
+  destruct a as [kn []]; cbn in * => //.
+  destruct Extract.E.cst_body => //. cbn in cla |- *.
+  now eapply EOptimizePropDiscr.closed_optimize.
+  now eapply EOptimizePropDiscr.closed_optimize.
+Qed.
+Next Obligation.
+  red. move=> fl [Σ t] /= v /andP[cle clt] [ev].
+  eapply EOptimizePropDiscr.optimize_correct in ev; eauto.
+  eexists; split => //. red. sq; auto.
+Qed.
