erasure/theories/EWcbvEvalEtaInd.v
@@ -1,7 +1,8 @@
 (* Distributed under the terms of the MIT license. *)
 From Coq Require Import Utf8 Program ssreflect ssrbool.
 From MetaCoq.Template Require Import config utils Kernames BasicAst EnvMap.
-From MetaCoq.Erasure Require Import EAst EAstUtils EInduction EWcbvEval EGlobalEnv ECSubst EInduction EWcbvEvalInd EEtaExpanded.
+From MetaCoq.Erasure Require Import EAst EAstUtils EInduction EWcbvEval EGlobalEnv
+   ECSubst EInduction EWcbvEvalInd EEtaExpanded.
 
 Set Asymmetric Patterns.
 From Equations Require Import Equations.
